Cleansup multiple files, remove old examples and tests, and states new lemmas.

Syntax.thy
@@ -15,7 +15,7 @@ begin
 lemma non_ac : 
   assumes \<open>label f \<noteq> AC\<close>
   shows \<open>label f = Unin \<or> label f = Hom\<close>
-using ach.exhaust assms by blast
+  using ach.exhaust assms by blast
 
 section \<open>Flattened Terms\<close>
 
@@ -31,53 +31,13 @@ inductive is_flattened :: "('f, 'v) term \<Rightarrow> bool" where
        \<And>t. t \<in> set ts \<Longrightarrow> is_flattened t;
        \<And>t g gs. t \<in> set ts \<Longrightarrow> t = Fun g gs \<Longrightarrow> g \<noteq> f \<rbrakk>  \<Longrightarrow> is_flattened (Fun f ts)"
 
-lemma test1_is_flattened:
-  assumes "label f = Unin"
-  shows "is_flattened (Fun f [Var x, Fun f [Var y, Var x]])"
-  by (metis ach.simps(2) assms empty_set fun_is_flattened list.simps(15) set_ConsD singletonD
-      var_is_flattened)
-
-
-lemma test2_is_flattened:
-  assumes "label f = AC"
-  shows "\<not> is_flattened (Fun f [Var x, Fun f [Var y, Var x]])"
-  using assms signature.is_flattened.cases by force
-
-value  "set [Var x, Fun g [Fun f [Var y, Var x], Var x]]"
-
-lemma example2:
-  assumes "label f = AC" and "label g = Unin"
-  shows "is_flattened (Fun f [Var x, Fun g [Fun f [Var y, Var x], Var x]])"
-  sorry
-
-(* Now we define a function that decides the above predicate *)
-
 fun is_headed_by_ac :: \<open>('f, 'v) term \<Rightarrow> bool\<close> where
-  \<open>is_headed_by_ac s =
-    (case s of
-      (Var _)   \<Rightarrow> False |
-      (Fun g _) \<Rightarrow> (case label g of
-        AC \<Rightarrow> True |
-        _  \<Rightarrow> False)
-    )\<close>
-
-lemma test_is_headed_by_ac:
-  assumes "label f = AC" and "label g = Unin"
-  shows "is_headed_by_ac (Fun f [Var x, Fun f [Var y, Var z]])"
-  using assms by simp
-
-lemma test_is_not_headed_by_ac:
-  assumes "label f = AC" and " label g = Hom"
-  shows "\<not> is_headed_by_ac (Fun g [Var x, Fun f [Var y, Var z]])"
-proof
-  assume H: "is_headed_by_ac (Fun g [Var x, Fun f [Var y, Var z]])"
-  from H have "(case label g of AC \<Rightarrow> True | _ \<Rightarrow> False)"
-    by simp
-  moreover from assms have "label g = Hom" 
-    by simp
-  ultimately show "False" by simp
-qed
-
+  \<open>is_headed_by_ac (Var _)   = False\<close> |
+  \<open>is_headed_by_ac (Fun g _) = (
+    case label g of
+      AC \<Rightarrow> True |
+      _  \<Rightarrow> False
+  )\<close>
 
 fun get_fun_symb :: \<open>('f, 'v) term \<Rightarrow> 'f option \<close> where
   \<open>get_fun_symb (Var _ )  = None\<close> |
@@ -92,110 +52,34 @@ fun dec_is_flattened :: \<open>('f, 'v) term \<Rightarrow> bool\<close> where
     (case label f of
       AC \<Rightarrow> (
         let ac_arg =
-          find
-            (\<lambda> s. (is_headed_by_ac s) \<and> (case (get_fun_symb s) of None \<Rightarrow> False | Some g \<Rightarrow> f = g))
-            ts
+          find (
+            \<lambda> s. (is_headed_by_ac s) \<and>
+            (case (get_fun_symb s) of None \<Rightarrow> False | Some g \<Rightarrow> f = g)
+          ) ts
         in
         (case ac_arg of
-          None \<Rightarrow> foldl (\<and>) True (map dec_is_flattened ts) |
-          Some _ \<Rightarrow> False)
-    )|
+          None   \<Rightarrow> foldl (\<and>) True (map dec_is_flattened ts) |
+          Some _ \<Rightarrow> False
+        )
+      )|
       _  \<Rightarrow> foldl (\<and>) True (map dec_is_flattened ts)
     )\<close>
 
-(*
-Note:
- 1. The repeated "foldl (\<and>) True (map dec_is_flattened ts)" is for efficiency reasons, we only compute
-  this foldl when strictly necessary, that's why there is no let ... in construct computing it
-  beforehand, as some branches of the function wouldn't need it.
- 2. Notice that on Line 105, there is no way that (is_headed_by_ac s) is true and the second component is false.
-    Since to be headed by AC you need to be of functional application form.
-    I cannot express this at the type level and Isabelle doesn't seem to subscribe to the "propositions as types" idea.
-*)
-
-lemma test_dec_is_flattened:
-  assumes "label f = AC"
-  shows "\<not> dec_is_flattened (Fun f [Var x, Fun f [Var y, Var z]])"
-  using assms by simp
-
-text \<open> The following should not be possible to prove. \<close>
-lemma test1_dec_is_flattened:
-  assumes "label f = AC" and "label g = Hom"
-  shows "\<not> dec_is_flattened (Fun f [Var x, Fun g [Var y, Fun f [Var z, Fun f [Var z, Var x]]]])"
-  apply (auto)
-  apply (simp add: assms)
-  done
-  
-
-lemma dec_pred_flatten:
-  assumes "is_flattened s"
-  shows " dec_is_flattened s"
-  apply (induction s)
-   apply (simp)
+lemma dec_pred_is_flatten: \<open>\<forall> s :: ('f, 'v) term. is_flatenned s \<longleftrightarrow> dec_is_flatened s\<close>
   sorry
 
-lemma dec_pred_is_flatten:
-  "is_flattened s \<longleftrightarrow> dec_is_flattened s" (is "?L \<longleftrightarrow> ?R ")
-  sorry
-
-(*proof (cases s)
-  case (Var x)
-  then show ?thesis
-    using Var var_is_flattened by fastforce
-next
-case (Fun f ts)
-  then show ?thesis
-  proof
-    assume H: "is_flattened (Fun f ts)"
-    from H show ?thesis
-      unfolding dec_is_flattened_def
-    proof (cases "label f = AC")
-      case True
-      (* AC case: use your ac_is_flattened rule / elimination to match
-         the condition that dec_is_flattened checks for AC-symbols *)
-      from H True show ?thesis
-        by (auto elim: is_flattened.cases)
-    next
-      case False
-      (* non-AC case: use fun_is_flattened + IH on all arguments *)
-      from H False show ?thesis
-        by (auto elim: is_flattened.cases)
-    qed
-  next
-    assume H: "dec_is_flattened (Fun f ts)"
-    show "is_flattened (Fun f ts)"
-      unfolding dec_is_flattened_def
-    proof (cases "label f = AC")
-      case True
-      (* AC case: build an is_flattened proof using ac_is_flattened *)
-      from H True show ?thesis
-        by (auto intro: is_flattened.intros)
-    next
-      case False
-      (* non-AC case: use fun_is_flattened and IH on arguments *)
-      from H False show ?thesis
-        by (auto intro: is_flattened.intros)
-    qed
-  qed
-qed
-*)
-
-
-text \<open>We define a function that flattens a term\<close>
+subsection "Flattening"
 
 fun flatten_aux :: \<open>'f \<Rightarrow> ('f, 'v) term \<Rightarrow> ('f, 'v) term list\<close> where
   \<open>flatten_aux f s =
-  (case s of
-    Var _ \<Rightarrow> [s] |
-    Fun g ss \<Rightarrow> (
-      (if label g = AC \<and> g = f then
-        args s
-      else
-        [s]
-      )
-    )
-  )
-  \<close>
+    (case s of
+      Var _    \<Rightarrow> [s] |
+      Fun g ss \<Rightarrow>
+        if label g = AC \<and> g = f then
+          args s
+        else
+          [s]
+    )\<close>
 
 
 fun flatten :: \<open>('f, 'v) term \<Rightarrow> ('f, 'v) term\<close> where
@@ -355,7 +239,7 @@ proof
           using flatten_AC_args_flattened Fun.hyps True by blast
         show "\<And>t g gs. t \<in> set (concat (map (flatten_aux f) (map flatten ss))) \<Longrightarrow> t = Fun g gs \<Longrightarrow> g \<noteq> f"
           using flatten_AC_no_nested Fun.hyps True
-            by blast  
+            by blast
         qed
     next
       case False
@@ -370,37 +254,28 @@ proof
 qed
 
 lemma flatten_soundness_dec: \<open>\<forall> t::('f, 'v) term. dec_is_flattened (flatten t)\<close>
-  using dec_pred_is_flatten flatten_soundness by fast
-
-lemma flatten_idempotent: \<open>flatten (flatten t) = t\<close>
-  sorry
+  using dec_pred_is_flatten flatten_soundness by blast
 
 (* this lemma seems necessary for proofs using equality *)
 lemma flatten_soundess_eq_form: \<open>is_flattened t \<longleftrightarrow> dec_is_flattened t = True\<close>
   sorry
 
+lemma flatten_idempotent: \<open>flatten (flatten t) = flatten t\<close>
+proof (induct t)
+  case (Var x)
+  then show ?case using var_is_flattened by simp
+next
+  case (Fun f ss)
+  then show ?case
+  proof (cases \<open>label f = AC\<close>)
+    case True
+    then show ?thesis
+      sorry
+  next
+    case False
+    then show ?thesis sorry
+  qed
+qed
 
-text \<open>O exemplo abaixo está com problema, agora esta certo\<close>
-
-lemma test1_Flatten:
-  assumes "label f = AC" and "label g = Hom"
-  shows "flatten (Fun f [Var z, Fun f [Var x, Var y]]) = Fun f [Var z, Var x, Var y]"
-  apply (simp add: assms)
-  done
-
-(* now this example and more complicated ones also work.
-  but to prove more complicated ones, one need to be able to correctly do the ordering.
-  - There is an interesting lemma in AC_equality.thy that says:
-  \<forall>s. ac_eq (flatten s) s, that is, every term is equal to its flattened form modulo AC.
- *)
-
-text \<open>This one is not possible because of the variable ordering\<close>
-lemma test2_Flatten:
-  assumes "label f = AC" 
-    and "label g = Hom"
-    and "x\<noteq>y"
-  shows "\<not>(flatten (Fun f [Var z, Fun f [Var x, Var y]]) = Fun f [Var x, Var y, Var y])"
-  apply (simp add: assms)
-  sorry
 end
 end
